src/AwsCryptographicMaterialProviders/Defaults.dfy
@@ -25,5 +25,6 @@ module {:extern "Defaults"} Defaults {
     if commitmentPolicy == Crypto.FORBID_ENCRYPT_ALLOW_DECRYPT then
       Crypto.ALG_AES_256_GCM_IV12_TAG16_HKDF_SHA384_ECDSA_P384 else
       Crypto.ALG_AES_256_GCM_IV12_TAG16_HKDF_SHA384_ECDSA_P384 // TODO: committing algorithm by default
+      //Crypto.ALG_AES_256_GCM_HKDF_SHA512_COMMIT_KEY_ECDSA_P384
   }
 }
