src/SDK/KeyDerivation.dfy
@@ -1,0 +1,149 @@
+include "../StandardLibrary/StandardLibrary.dfy"
+include "../StandardLibrary/UInt.dfy"
+include "../AwsCryptographicMaterialProviders/Client.dfy"
+include "../Crypto/HKDF/HKDF.dfy"
+include "../Crypto/HKDF/HMAC.dfy"
+
+include "Serialize/HeaderTypes.dfy"
+include "Serialize/SerializableTypes.dfy"
+
+
+module {:extern "KeyDerivation"} KeyDerivation {
+  import opened Wrappers
+  import opened UInt = StandardLibrary.UInt
+  import UTF8
+  import MaterialProviders.Client
+  import HeaderTypes
+  import SerializableTypes
+  import HKDF
+  import HMAC
+
+
+  // Convenience container to hold both K_e and K_c necessary
+  // for encryption with key commitment
+  datatype ExpandedKeyMaterial = ExpandedKeyMaterial(
+    nameonly dataKey: seq<uint8>,
+    nameonly commitmentKey: Option<seq<uint8>>
+  )
+
+  /*
+   * Derives a single data key from an input plaintext data key, using "v1"-style
+   * key derivation (that is, no key commitment).
+   */
+  method DeriveKey(
+    messageId: HeaderTypes.MessageID,
+    plaintextDataKey: seq<uint8>,
+    suite: Client.AlgorithmSuites.AlgorithmSuite
+  ) 
+    returns (res: Result<ExpandedKeyMaterial, string>)
+
+    requires |plaintextDataKey| == suite.encrypt.keyLength as int
+
+    ensures res.Success? ==> |res.value.dataKey| == suite.encrypt.keyLength as int
+    ensures res.Success? ==> IsDerivedKey(res.value.dataKey)
+  {
+    if suite.kdf.IDENTITY? {
+      assert IsDerivedKey(plaintextDataKey) by {
+        reveal IsDerivedKey();
+      }
+      return Success(ExpandedKeyMaterial(dataKey:=plaintextDataKey, commitmentKey:=None()));
+    }
+
+    var algorithmSuiteID := SerializableTypes.GetESDKAlgorithmSuiteId(suite.id);
+    var infoSeq := UInt16ToSeq(algorithmSuiteID as uint16) + messageId;
+    var len := suite.kdf.inputKeyLength as int;
+    var derivedKey := HKDF.Hkdf(suite.kdf.hmac, None, plaintextDataKey, infoSeq, len);
+    assert IsDerivedKey(derivedKey) by {
+      reveal IsDerivedKey();
+    }
+      return Success(ExpandedKeyMaterial(dataKey:=derivedKey, commitmentKey:=None()));
+  }
+
+  /*
+   * Derives keys from an input plaintext data key, using "v2"-style
+   * key derivation (that is, including key commitment).
+   */
+  method ExpandKeyMaterial(
+    messageId: HeaderTypes.MessageID,
+    plaintextKey: seq<uint8>,
+    suite: Client.AlgorithmSuites.AlgorithmSuiteInfo
+  )
+    returns (res: Result<ExpandedKeyMaterial, string>)
+
+    // This should only be used for algorithms with commitment
+    requires !suite.commitment.None?
+
+    requires |messageId| != 0
+    requires |plaintextKey| == suite.encrypt.keyLength as int
+    // TODO: seems like this should follow from the fact that |key| == keyLength,
+    // but apparently we don't prove/require any where that keys be small.
+    requires |plaintextKey| < INT32_MAX_LIMIT
+
+    // Make sure we return a commitment key
+    ensures
+      && res.Success?
+    ==>
+      res.value.commitmentKey.Some?
+  {
+    var KEY_LABEL :- UTF8.Encode("DERIVEKEY");
+    var COMMIT_LABEL :- UTF8.Encode("COMMITKEY");
+
+    //var digest := suite.commitment.hmac;
+    var digest := HMAC.SHA_512; // TODO
+    var esdkId := UInt.UInt16ToSeq(SerializableTypes.GetESDKAlgorithmSuiteId(suite.id));
+    var info := esdkId + KEY_LABEL;
+
+    var hmac1 := new HMAC.HMac(digest);
+    hmac1.Init(messageId);
+
+    var PRK := HKDF.Extract(hmac1, messageId, plaintextKey, hmac1.GetDigest());
+
+    // method Expand(
+      //hmac: HMac,
+      //prk: seq<uint8>,
+      //info: seq<uint8>,
+      //expectedLength: int,
+      //digest: Digests,
+      //ghost salt: seq<uint8>)
+      //returns (okm: seq<uint8>, ghost okmUnabridged: seq<uint8>)
+
+    var Ke, _ := HKDF.Expand(hmac1, PRK, info, suite.encrypt.keyLength as int, digest, messageId);
+
+    var hmac2 := new HMAC.HMac(digest);
+    hmac2.Init(messageId);
+
+    var Kc, _ := HKDF.Expand(hmac2, PRK, COMMIT_LABEL, suite.encrypt.keyLength as int, digest, messageId);
+
+    return Success(ExpandedKeyMaterial(dataKey:=Ke, commitmentKey:=Some(Kc)));
+  }
+
+  predicate {:opaque} IsDerivedKey(derivedDataKey: seq<uint8>)
+  {
+    true
+  }
+
+  /*
+   * Derives key material for encryption/decryption. Delegates out to specific methods
+   * based on the input algorithm suite.
+   */
+  method DeriveKeys(
+    messageId: HeaderTypes.MessageID,
+    plaintextKey: seq<uint8>,
+    suite: Client.AlgorithmSuites.AlgorithmSuite
+  )
+    returns (res: Result<ExpandedKeyMaterial, string>)
+
+    requires |messageId| != 0
+    requires |plaintextKey| == suite.encrypt.keyLength as int
+
+  {
+    var keys : ExpandedKeyMaterial;
+    if (!suite.commitment.None?) {
+      keys :- ExpandKeyMaterial(messageId, plaintextKey, suite);
+    } else {
+      keys :- DeriveKey(messageId, plaintextKey, suite);
+    }
+
+    return Success(keys);
+  }
+}
